A specific constructor for injecting values in expressions
We add a specific constructor to the type of expressions for injecting
values in expressions.

The advantage are :
- Values can be assumed to be always closed when performing
  substitutions (even though they could contain free variables, but it
  turns out it does not cause any problem in the proofs in
  practice). This means that we no longer need the `Closed` typeclass
  and everything that comes with it (all the reflection-based machinery
  contained in tactics.v is no longer necessary). I have not measured
  anything, but I guess this would have a significant performance
  impact.

- There is only one constructor for values. As a result, the AsVal and
  IntoVal typeclasses are no longer necessary: an expression which is
  a value will always unify with `Val _`, and therefore lemmas can be
  stated using this constructor.

Of course, this means that there are two ways of writing such a thing
as "The pair of integers 1 and 2": Either by using the value
constructor applied to the pair represented as a value, or by using
the expression pair constructor. So we add reduction rules that
transform reduced pair, injection and closure expressions into values.
At first, this seems weird, because of the redundancy. But in fact,
this has some meaning, since the machine migth actually be doing
something to e.g., allocate the pair or the closure.

These additional steps of computation show up in the proofs, and some
additional wp_* tactics need to be called.

theories/heap_lang/lifting.v
@@ -44,7 +44,6 @@ Ltac inv_head_step :=
      inversion H; subst; clear H
   end.
 
-Local Hint Extern 0 (atomic _ _) => solve_atomic.
 Local Hint Extern 0 (head_reducible _ _) => eexists _, _, _, _; simpl.
 Local Hint Extern 0 (head_reducible_no_obs _ _) => eexists _, _, _; simpl.
 
@@ -59,51 +58,61 @@ Local Hint Resolve to_of_val.
 Local Ltac solve_exec_safe := intros; subst; do 3 eexists; econstructor; eauto.
 Local Ltac solve_exec_puredet := simpl; intros; by inv_head_step.
 Local Ltac solve_pure_exec :=
-  unfold IntoVal in *;
-  repeat match goal with H : AsVal _ |- _ => destruct H as [??] end; subst;
-  intros ?; apply nsteps_once, pure_head_step_pure_step;
+  subst; intros ?; apply nsteps_once, pure_head_step_pure_step;
     constructor; [solve_exec_safe | solve_exec_puredet].
 
-Class AsRec (e : expr) (f x : binder) (erec : expr) :=
-  as_rec : e = Rec f x erec.
-Instance AsRec_rec f x e : AsRec (Rec f x e) f x e := eq_refl.
-Instance AsRec_rec_locked_val v f x e :
-  AsRec (of_val v) f x e → AsRec (of_val (locked v)) f x e.
+Class AsRecV (v : val) (f x : binder) (erec : expr) :=
+  as_recv : v = RecV f x erec.
+Instance AsRecV_recv f x e : AsRecV (RecV f x e) f x e := eq_refl.
+Instance AsRecV_recv_locked v f x e :
+  AsRecV v f x e → AsRecV (locked v) f x e.
 Proof. by unlock. Qed.
 
-Instance pure_rec f x (erec e1 e2 : expr)
-    `{!AsVal e2, AsRec e1 f x erec, Closed (f :b: x :b: []) erec} :
-  PureExec True 1 (App e1 e2) (subst' x e2 (subst' f e1 erec)).
-Proof. unfold AsRec in *; solve_pure_exec. Qed.
-
-Instance pure_unop op e v v' `{!IntoVal e v} :
-  PureExec (un_op_eval op v = Some v') 1 (UnOp op e) (of_val v').
+Instance pure_recc f x (erec : expr) :
+  PureExec True 1 (Rec f x erec) (Val $ RecV f x erec).
+Proof. solve_pure_exec. Qed.
+Instance pure_pairc (v1 v2 : val) :
+  PureExec True 1 (Pair (Val v1) (Val v2)) (Val $ PairV v1 v2).
+Proof. solve_pure_exec. Qed.
+Instance pure_injlc (v : val) :
+  PureExec True 1 (InjL $ Val v) (Val $ InjLV v).
+Proof. solve_pure_exec. Qed.
+Instance pure_injrc (v : val) :
+  PureExec True 1 (InjR $ Val v) (Val $ InjRV v).
 Proof. solve_pure_exec. Qed.
 
-Instance pure_binop op e1 e2 v1 v2 v' `{!IntoVal e1 v1, !IntoVal e2 v2} :
-  PureExec (bin_op_eval op v1 v2 = Some v') 1 (BinOp op e1 e2) (of_val v').
+Instance pure_beta f x (erec : expr) (v1 v2 : val) `{AsRecV v1 f x erec} :
+  PureExec True 1 (App (Val v1) (Val v2)) (subst' x v2 (subst' f v1 erec)).
+Proof. unfold AsRecV in *. solve_pure_exec. Qed.
+
+Instance pure_unop op v v' :
+  PureExec (un_op_eval op v = Some v') 1 (UnOp op (Val v)) (Val v').
 Proof. solve_pure_exec. Qed.
 
-Instance pure_if_true e1 e2 : PureExec True 1 (If (Lit (LitBool true)) e1 e2) e1.
+Instance pure_binop op v1 v2 v' :
+  PureExec (bin_op_eval op v1 v2 = Some v') 1 (BinOp op (Val v1) (Val v2)) (Val v').
 Proof. solve_pure_exec. Qed.
 
-Instance pure_if_false e1 e2 : PureExec True 1 (If (Lit (LitBool false)) e1 e2) e2.
+Instance pure_if_true e1 e2 : PureExec True 1 (If (Val $ LitV $ LitBool true) e1 e2) e1.
 Proof. solve_pure_exec. Qed.
 
-Instance pure_fst e1 e2 v1 `{!IntoVal e1 v1, !AsVal e2} :
-  PureExec True 1 (Fst (Pair e1 e2)) e1.
+Instance pure_if_false e1 e2 : PureExec True 1 (If (Val $ LitV  $ LitBool false) e1 e2) e2.
 Proof. solve_pure_exec. Qed.
 
-Instance pure_snd e1 e2 v2 `{!AsVal e1, !IntoVal e2 v2} :
-  PureExec True 1 (Snd (Pair e1 e2)) e2.
+Instance pure_fst v1 v2 :
+  PureExec True 1 (Fst (Val $ PairV v1 v2)) (Val v1).
 Proof. solve_pure_exec. Qed.
 
-Instance pure_case_inl e0 v e1 e2 `{!IntoVal e0 v} :
-  PureExec True 1 (Case (InjL e0) e1 e2) (App e1 e0).
+Instance pure_snd v1 v2 :
+  PureExec True 1 (Snd (Val $ PairV v1 v2)) (Val v2).
 Proof. solve_pure_exec. Qed.
 
-Instance pure_case_inr e0 v e1 e2 `{!IntoVal e0 v} :
-  PureExec True 1 (Case (InjR e0) e1 e2) (App e2 e0).
+Instance pure_case_inl v e1 e2 :
+  PureExec True 1 (Case (Val $ InjLV v) e1 e2) (App e1 (Val v)).
+Proof. solve_pure_exec. Qed.
+
+Instance pure_case_inr v e1 e2 :
+  PureExec True 1 (Case (Val $ InjRV v) e1 e2) (App e2 (Val v)).
 Proof. solve_pure_exec. Qed.
 
 Section lifting.
@@ -131,21 +140,19 @@ Proof.
 Qed.
 
 (** Heap *)
-Lemma wp_alloc s E e v :
-  IntoVal e v →
-  {{{ True }}} Alloc e @ s; E {{{ l, RET LitV (LitLoc l); l ↦ v }}}.
+Lemma wp_alloc s E v :
+  {{{ True }}} Alloc (Val v) @ s; E {{{ l, RET LitV (LitLoc l); l ↦ v }}}.
 Proof.
-  iIntros (<- Φ) "_ HΦ". iApply wp_lift_atomic_head_step_no_fork; auto.
-  iIntros (σ1 κ κs) "[Hσ Hκs] !>"; iSplit; first by eauto.
+  iIntros (Φ) "_ HΦ". iApply wp_lift_atomic_head_step_no_fork; auto.
+  iIntros (σ1 κ κs) "[Hσ Hκs] !>"; iSplit; first by auto.
   iNext; iIntros (v2 σ2 efs Hstep); inv_head_step.
   iMod (@gen_heap_alloc with "Hσ") as "[Hσ Hl]"; first done.
   iModIntro; iSplit=> //. iFrame. by iApply "HΦ".
 Qed.
-Lemma twp_alloc s E e v :
-  IntoVal e v →
-  [[{ True }]] Alloc e @ s; E [[{ l, RET LitV (LitLoc l); l ↦ v }]].
+Lemma twp_alloc s E v :
+  [[{ True }]] Alloc (Val v) @ s; E [[{ l, RET LitV (LitLoc l); l ↦ v }]].
 Proof.
-  iIntros (<- Φ) "_ HΦ". iApply twp_lift_atomic_head_step_no_fork; auto.
+  iIntros (Φ) "_ HΦ". iApply twp_lift_atomic_head_step_no_fork; auto.
   iIntros (σ1 κs) "[Hσ Hκs] !>"; iSplit; first by eauto.
   iIntros (κ v2 σ2 efs Hstep); inv_head_step.
   iMod (@gen_heap_alloc with "Hσ") as "[Hσ Hl]"; first done.
@@ -153,7 +160,7 @@ Proof.
 Qed.
 
 Lemma wp_load s E l q v :
-  {{{ ▷ l ↦{q} v }}} Load (Lit (LitLoc l)) @ s; E {{{ RET v; l ↦{q} v }}}.
+  {{{ ▷ l ↦{q} v }}} Load (Val $ LitV $ LitLoc l) @ s; E {{{ RET v; l ↦{q} v }}}.
 Proof.
   iIntros (Φ) ">Hl HΦ". iApply wp_lift_atomic_head_step_no_fork; auto.
   iIntros (σ1 κ κs) "[Hσ Hκs] !>". iDestruct (@gen_heap_valid with "Hσ Hl") as %?.
@@ -161,7 +168,7 @@ Proof.
   iModIntro; iSplit=> //. iFrame. by iApply "HΦ".
 Qed.
 Lemma twp_load s E l q v :
-  [[{ l ↦{q} v }]] Load (Lit (LitLoc l)) @ s; E [[{ RET v; l ↦{q} v }]].
+  [[{ l ↦{q} v }]] Load (Val $ LitV $ LitLoc l) @ s; E [[{ RET v; l ↦{q} v }]].
 Proof.
   iIntros (Φ) "Hl HΦ". iApply twp_lift_atomic_head_step_no_fork; auto.
   iIntros (σ1 κs) "[Hσ Hκs] !>". iDestruct (@gen_heap_valid with "Hσ Hl") as %?.
@@ -169,22 +176,22 @@ Proof.
   iModIntro; iSplit=> //. iSplit; first done. iFrame. by iApply "HΦ".
 Qed.
 
-Lemma wp_store s E l v' e v :
-  IntoVal e v →
-  {{{ ▷ l ↦ v' }}} Store (Lit (LitLoc l)) e @ s; E {{{ RET LitV LitUnit; l ↦ v }}}.
+Lemma wp_store s E l v' v :
+  {{{ ▷ l ↦ v' }}} Store (Val $ LitV (LitLoc l)) (Val v) @ s; E
+  {{{ RET LitV LitUnit; l ↦ v }}}.
 Proof.
-  iIntros (<- Φ) ">Hl HΦ".
+  iIntros (Φ) ">Hl HΦ".
   iApply wp_lift_atomic_head_step_no_fork; auto.
   iIntros (σ1 κ κs) "[Hσ Hκs] !>". iDestruct (@gen_heap_valid with "Hσ Hl") as %?.
   iSplit; first by eauto. iNext; iIntros (v2 σ2 efs Hstep); inv_head_step.
   iMod (@gen_heap_update with "Hσ Hl") as "[$ Hl]".
   iModIntro. iSplit=>//. iFrame. by iApply "HΦ".
 Qed.
-Lemma twp_store s E l v' e v :
-  IntoVal e v →
-  [[{ l ↦ v' }]] Store (Lit (LitLoc l)) e @ s; E [[{ RET LitV LitUnit; l ↦ v }]].
+Lemma twp_store s E l v' v :
+  [[{ l ↦ v' }]] Store (Val $ LitV $ LitLoc l) (Val v) @ s; E
+  [[{ RET LitV LitUnit; l ↦ v }]].
 Proof.
-  iIntros (<- Φ) "Hl HΦ".
+  iIntros (Φ) "Hl HΦ".
   iApply twp_lift_atomic_head_step_no_fork; auto.
   iIntros (σ1 κs) "[Hσ Hκs] !>". iDestruct (@gen_heap_valid with "Hσ Hl") as %?.
   iSplit; first by eauto. iIntros (κ v2 σ2 efs Hstep); inv_head_step.
@@ -192,73 +199,65 @@ Proof.
   iModIntro. iSplit=>//. iSplit; first done. iFrame. by iApply "HΦ".
 Qed.
 
-Lemma wp_cas_fail s E l q v' e1 v1 e2 :
-  IntoVal e1 v1 → AsVal e2 → v' ≠ v1 → vals_cas_compare_safe v' v1 →
-  {{{ ▷ l ↦{q} v' }}} CAS (Lit (LitLoc l)) e1 e2 @ s; E
+Lemma wp_cas_fail s E l q v' v1 v2 :
+  v' ≠ v1 → vals_cas_compare_safe v' v1 →
+  {{{ ▷ l ↦{q} v' }}} CAS (Val $ LitV $ LitLoc l) (Val v1) (Val v2) @ s; E
   {{{ RET LitV (LitBool false); l ↦{q} v' }}}.
 Proof.
-  iIntros (<- [v2 <-] ?? Φ) ">Hl HΦ".
-  iApply wp_lift_atomic_head_step_no_fork; auto.
+  iIntros (?? Φ) ">Hl HΦ". iApply wp_lift_atomic_head_step_no_fork; auto.
   iIntros (σ1 κ κs) "[Hσ Hκs] !>". iDestruct (@gen_heap_valid with "Hσ Hl") as %?.
   iSplit; first by eauto. iNext; iIntros (v2' σ2 efs Hstep); inv_head_step.
   iModIntro; iSplit=> //. iFrame. by iApply "HΦ".
 Qed.
-Lemma twp_cas_fail s E l q v' e1 v1 e2 :
-  IntoVal e1 v1 → AsVal e2 → v' ≠ v1 → vals_cas_compare_safe v' v1 →
-  [[{ l ↦{q} v' }]] CAS (Lit (LitLoc l)) e1 e2 @ s; E
+Lemma twp_cas_fail s E l q v' v1 v2 :
+  v' ≠ v1 → vals_cas_compare_safe v' v1 →
+  [[{ l ↦{q} v' }]] CAS (Val $ LitV $ LitLoc l) (Val v1) (Val v2) @ s; E
   [[{ RET LitV (LitBool false); l ↦{q} v' }]].
 Proof.
-  iIntros (<- [v2 <-] ?? Φ) "Hl HΦ".
-  iApply twp_lift_atomic_head_step_no_fork; auto.
+  iIntros (?? Φ) "Hl HΦ". iApply twp_lift_atomic_head_step_no_fork; auto.
   iIntros (σ1 κs) "[Hσ Hκs] !>". iDestruct (@gen_heap_valid with "Hσ Hl") as %?.
   iSplit; first by eauto. iIntros (κ v2' σ2 efs Hstep); inv_head_step.
   iModIntro; iSplit=> //. iSplit; first done. iFrame. by iApply "HΦ".
 Qed.
 
-Lemma wp_cas_suc s E l e1 v1 e2 v2 :
-  IntoVal e1 v1 → IntoVal e2 v2 → vals_cas_compare_safe v1 v1 →
-  {{{ ▷ l ↦ v1 }}} CAS (Lit (LitLoc l)) e1 e2 @ s; E
+Lemma wp_cas_suc s E l v1 v2 :
+  vals_cas_compare_safe v1 v1 →
+  {{{ ▷ l ↦ v1 }}} CAS (Val $ LitV $ LitLoc l) (Val v1) (Val v2) @ s; E
   {{{ RET LitV (LitBool true); l ↦ v2 }}}.
 Proof.
-  iIntros (<- <- ? Φ) ">Hl HΦ".
-  iApply wp_lift_atomic_head_step_no_fork; auto.
+  iIntros (? Φ) ">Hl HΦ". iApply wp_lift_atomic_head_step_no_fork; auto.
   iIntros (σ1 κ κs) "[Hσ Hκs] !>". iDestruct (@gen_heap_valid with "Hσ Hl") as %?.
   iSplit; first by eauto. iNext; iIntros (v2' σ2 efs Hstep); inv_head_step.
   iMod (@gen_heap_update with "Hσ Hl") as "[$ Hl]".
   iModIntro. iSplit=>//. iFrame. by iApply "HΦ".
 Qed.
-Lemma twp_cas_suc s E l e1 v1 e2 v2 :
-  IntoVal e1 v1 → IntoVal e2 v2 → vals_cas_compare_safe v1 v1 →
-  [[{ l ↦ v1 }]] CAS (Lit (LitLoc l)) e1 e2 @ s; E
+Lemma twp_cas_suc s E l v1 v2 :
+  vals_cas_compare_safe v1 v1 →
+  [[{ l ↦ v1 }]] CAS (Val $ LitV $ LitLoc l) (Val v1) (Val v2) @ s; E
   [[{ RET LitV (LitBool true); l ↦ v2 }]].
 Proof.
-  iIntros (<- <- ? Φ) "Hl HΦ".
-  iApply twp_lift_atomic_head_step_no_fork; auto.
+  iIntros (? Φ) "Hl HΦ". iApply twp_lift_atomic_head_step_no_fork; auto.
   iIntros (σ1 κs) "[Hσ Hκs] !>". iDestruct (@gen_heap_valid with "Hσ Hl") as %?.
   iSplit; first by eauto. iIntros (κ v2' σ2 efs Hstep); inv_head_step.
   iMod (@gen_heap_update with "Hσ Hl") as "[$ Hl]".
   iModIntro. iSplit=>//. iSplit; first done. iFrame. by iApply "HΦ".
 Qed.
 
-Lemma wp_faa s E l i1 e2 i2 :
-  IntoVal e2 (LitV (LitInt i2)) →
-  {{{ ▷ l ↦ LitV (LitInt i1) }}} FAA (Lit (LitLoc l)) e2 @ s; E
+Lemma wp_faa s E l i1 i2 :
+  {{{ ▷ l ↦ LitV (LitInt i1) }}} FAA (Val $ LitV $ LitLoc l) (Val $ LitV $ LitInt i2) @ s; E
   {{{ RET LitV (LitInt i1); l ↦ LitV (LitInt (i1 + i2)) }}}.
 Proof.
-  iIntros (<- Φ) ">Hl HΦ".
-  iApply wp_lift_atomic_head_step_no_fork; auto.
+  iIntros (Φ) ">Hl HΦ". iApply wp_lift_atomic_head_step_no_fork; auto.
   iIntros (σ1 κ κs) "[Hσ Hκs] !>". iDestruct (@gen_heap_valid with "Hσ Hl") as %?.
   iSplit; first by eauto. iNext; iIntros (v2' σ2 efs Hstep); inv_head_step.
   iMod (@gen_heap_update with "Hσ Hl") as "[$ Hl]".
   iModIntro. iSplit=>//. iFrame. by iApply "HΦ".
 Qed.
-Lemma twp_faa s E l i1 e2 i2 :
-  IntoVal e2 (LitV (LitInt i2)) →
-  [[{ l ↦ LitV (LitInt i1) }]] FAA (Lit (LitLoc l)) e2 @ s; E
+Lemma twp_faa s E l i1 i2 :
+  [[{ l ↦ LitV (LitInt i1) }]] FAA (Val $ LitV $ LitLoc l) (Val $ LitV $ LitInt i2) @ s; E
   [[{ RET LitV (LitInt i1); l ↦ LitV (LitInt (i1 + i2)) }]].
 Proof.
-  iIntros (<- Φ) "Hl HΦ".
-  iApply twp_lift_atomic_head_step_no_fork; auto.
+  iIntros (Φ) "Hl HΦ". iApply twp_lift_atomic_head_step_no_fork; auto.
   iIntros (σ1 κs) "[Hσ Hκs] !>". iDestruct (@gen_heap_valid with "Hσ Hl") as %?.
   iSplit; first by eauto. iIntros (κ e2 σ2 efs Hstep); inv_head_step.
   iMod (@gen_heap_update with "Hσ Hl") as "[$ Hl]".
