theories/heap_lang/lib/increment.v
@@ -23,15 +23,14 @@ Section increment.
   Lemma incr_spec (l: loc) :
     <<< ∀ (v : Z), l ↦ #v >>> incr #l @ ⊤ <<< l ↦ #(v + 1), RET #v >>>.
   Proof.
-    iApply wp_atomic_intro. iIntros (Φ) "AU". iLöb as "IH". wp_let.
+    iApply wp_atomic_intro. iIntros (Φ) "AU". iLöb as "IH". wp_lam.
     wp_apply load_spec; first by iAccu.
     (* Prove the atomic update for load *)
     iAuIntro. iApply (aacc_aupd_abort with "AU"); first done.
     iIntros (x) "H↦". iAaccIntro with "H↦"; first by eauto with iFrame.
     iIntros "$ !> AU !> _".
     (* Now go on *)
-    wp_let. wp_op. wp_bind (CAS _ _ _)%I.
-    wp_apply cas_spec; [done|iAccu|].
+    wp_let. wp_op. wp_apply cas_spec; [done|iAccu|].
     (* Prove the atomic update for CAS *)
     iAuIntro. iApply (aacc_aupd with "AU"); first done.
     iIntros (x') "H↦". iAaccIntro with "H↦"; first by eauto with iFrame.
@@ -57,7 +56,7 @@ Section increment.
       weak_incr #l @ ⊤
     <<< ⌜v = v'⌝ ∗ l ↦ #(v + 1), RET #v >>>.
   Proof.
-    iIntros "Hl". iApply wp_atomic_intro. iIntros (Φ) "AU". wp_let.
+    iIntros "Hl". iApply wp_atomic_intro. iIntros (Φ) "AU". wp_lam.
     wp_apply (atomic_wp_seq $! (load_spec _) with "Hl").
     iIntros "Hl". wp_let. wp_op.
     wp_apply store_spec; first by iAccu.
@@ -86,7 +85,7 @@ Section increment_client.
   Lemma incr_client_safe (x: Z):
     WP incr_client #x {{ _, True }}%I.
   Proof using Type*.
-    wp_let. wp_alloc l as "Hl". wp_let.
+    wp_lam. wp_alloc l as "Hl". wp_let.
     iMod (inv_alloc nroot _ (∃x':Z, l ↦ #x')%I with "[Hl]") as "#Hinv"; first eauto.
     (* FIXME: I am only using persistent stuff, so I should be allowed
        to move this to the persisten context even without the additional □. *)
