theories/heap_lang/proofmode.v
@@ -28,7 +28,6 @@ Tactic Notation "wp_expr_eval" tactic(t) :=
   end.
 
 Ltac wp_expr_simpl := wp_expr_eval simpl.
-Ltac wp_expr_simpl_subst := wp_expr_eval simpl_subst.
 
 Lemma tac_wp_pure `{heapG Σ} Δ Δ' s E e1 e2 φ n Φ :
   PureExec φ n e1 e2 →
@@ -49,19 +48,15 @@ Proof.
   rewrite envs_entails_eq=> ?? ->. rewrite -total_lifting.twp_pure_step //.
 Qed.
 
-Lemma tac_wp_value `{heapG Σ} Δ s E Φ e v :
-  IntoVal e v →
-  envs_entails Δ (Φ v) → envs_entails Δ (WP e @ s; E {{ Φ }}).
-Proof. rewrite envs_entails_eq=> ? ->. by apply wp_value. Qed.
-Lemma tac_twp_value `{heapG Σ} Δ s E Φ e v :
-  IntoVal e v →
-  envs_entails Δ (Φ v) → envs_entails Δ (WP e @ s; E [{ Φ }]).
-Proof. rewrite envs_entails_eq=> ? ->. by apply twp_value. Qed.
+Lemma tac_wp_value `{heapG Σ} Δ s E Φ v :
+  envs_entails Δ (Φ v) → envs_entails Δ (WP (Val v) @ s; E {{ Φ }}).
+Proof. rewrite envs_entails_eq=> ->. by apply wp_value. Qed.
+Lemma tac_twp_value `{heapG Σ} Δ s E Φ v :
+  envs_entails Δ (Φ v) → envs_entails Δ (WP (Val v) @ s; E [{ Φ }]).
+Proof. rewrite envs_entails_eq=> ->. by apply twp_value. Qed.
 
 Ltac wp_value_head :=
-  first [eapply tac_wp_value || eapply tac_twp_value];
-    [iSolveTC
-    |reduction.pm_prettify; iEval (simpl of_val)].
+  first [eapply tac_wp_value || eapply tac_twp_value]; reduction.pm_prettify.
 
 Tactic Notation "wp_pure" open_constr(efoc) :=
   iStartProof;
@@ -74,7 +69,7 @@ Tactic Notation "wp_pure" open_constr(efoc) :=
       [iSolveTC                       (* PureExec *)
       |try fast_done                  (* The pure condition for PureExec *)
       |iSolveTC                       (* IntoLaters *)
-      |wp_expr_simpl_subst; try wp_value_head (* new goal *)
+      |wp_expr_simpl; try wp_value_head (* new goal *)
       ])
     || fail "wp_pure: cannot find" efoc "in" e "or" efoc "is not a redex"
   | |- envs_entails _ (twp ?s ?E ?e ?Q) =>
@@ -84,34 +79,37 @@ Tactic Notation "wp_pure" open_constr(efoc) :=
       eapply (tac_twp_pure _ _ _ (fill K e'));
       [iSolveTC                       (* PureExec *)
       |try fast_done                  (* The pure condition for PureExec *)
-      |wp_expr_simpl_subst; try wp_value_head (* new goal *)
+      |wp_expr_simpl; try wp_value_head (* new goal *)
       ])
     || fail "wp_pure: cannot find" efoc "in" e "or" efoc "is not a redex"
   | _ => fail "wp_pure: not a 'wp'"
   end.
 
 Tactic Notation "wp_if" := wp_pure (If _ _ _).
-Tactic Notation "wp_if_true" := wp_pure (If (Lit (LitBool true)) _ _).
-Tactic Notation "wp_if_false" := wp_pure (If (Lit (LitBool false)) _ _).
+Tactic Notation "wp_if_true" := wp_pure (If (LitV (LitBool true)) _ _).
+Tactic Notation "wp_if_false" := wp_pure (If (LitV (LitBool false)) _ _).
 Tactic Notation "wp_unop" := wp_pure (UnOp _ _).
 Tactic Notation "wp_binop" := wp_pure (BinOp _ _ _).
 Tactic Notation "wp_op" := wp_unop || wp_binop.
 Tactic Notation "wp_rec" := wp_pure (App _ _).
 Tactic Notation "wp_lam" := wp_rec.
-Tactic Notation "wp_let" := wp_lam.
-Tactic Notation "wp_seq" := wp_lam.
+Tactic Notation "wp_let" := wp_pure (Rec BAnon (BNamed _) _); wp_lam.
+Tactic Notation "wp_seq" := wp_pure (Rec BAnon BAnon _); wp_lam.
 Tactic Notation "wp_proj" := wp_pure (Fst _) || wp_pure (Snd _).
 Tactic Notation "wp_case" := wp_pure (Case _ _ _).
-Tactic Notation "wp_match" := wp_case; wp_let.
+Tactic Notation "wp_match" := wp_case; wp_pure (Rec _ _ _); wp_lam.
+Tactic Notation "wp_inj" := wp_pure (InjL _) || wp_pure (InjR _).
+Tactic Notation "wp_pair" := wp_pure (Pair _ _).
+Tactic Notation "wp_closure" := wp_pure (Rec _ _ _).
 
 Lemma tac_wp_bind `{heapG Σ} K Δ s E Φ e f :
   f = (λ e, fill K e) → (* as an eta expanded hypothesis so that we can `simpl` it *)
-  envs_entails Δ (WP e @ s; E {{ v, WP f (of_val v) @ s; E {{ Φ }} }})%I →
+  envs_entails Δ (WP e @ s; E {{ v, WP f (Val v) @ s; E {{ Φ }} }})%I →
   envs_entails Δ (WP fill K e @ s; E {{ Φ }}).
 Proof. rewrite envs_entails_eq=> -> ->. by apply: wp_bind. Qed.
 Lemma tac_twp_bind `{heapG Σ} K Δ s E Φ e f :
   f = (λ e, fill K e) → (* as an eta expanded hypothesis so that we can `simpl` it *)
-  envs_entails Δ (WP e @ s; E [{ v, WP f (of_val v) @ s; E [{ Φ }] }])%I →
+  envs_entails Δ (WP e @ s; E [{ v, WP f (Val v) @ s; E [{ Φ }] }])%I →
   envs_entails Δ (WP fill K e @ s; E [{ Φ }]).
 Proof. rewrite envs_entails_eq=> -> ->. by apply: twp_bind. Qed.
 
@@ -144,29 +142,29 @@ Context `{heapG Σ}.
 Implicit Types P Q : iProp Σ.
 Implicit Types Φ : val → iProp Σ.
 Implicit Types Δ : envs (uPredI (iResUR Σ)).
+Implicit Types v : val.
+Implicit Types z : Z.
 
-Lemma tac_wp_alloc Δ Δ' s E j K e v Φ :
-  IntoVal e v →
+Lemma tac_wp_alloc Δ Δ' s E j K v Φ :
   MaybeIntoLaterNEnvs 1 Δ Δ' →
   (∀ l, ∃ Δ'',
     envs_app false (Esnoc Enil j (l ↦ v)) Δ' = Some Δ'' ∧
-    envs_entails Δ'' (WP fill K (Lit (LitLoc l)) @ s; E {{ Φ }})) →
-  envs_entails Δ (WP fill K (Alloc e) @ s; E {{ Φ }}).
+    envs_entails Δ'' (WP fill K (Val $ LitV l) @ s; E {{ Φ }})) →
+  envs_entails Δ (WP fill K (Alloc v) @ s; E {{ Φ }}).
 Proof.
-  rewrite envs_entails_eq=> ?? HΔ.
+  rewrite envs_entails_eq=> ? HΔ.
   rewrite -wp_bind. eapply wand_apply; first exact: wp_alloc.
   rewrite left_id into_laterN_env_sound; apply later_mono, forall_intro=> l.
   destruct (HΔ l) as (Δ''&?&HΔ'). rewrite envs_app_sound //; simpl.
   by rewrite right_id HΔ'.
 Qed.
-Lemma tac_twp_alloc Δ s E j K e v Φ :
-  IntoVal e v →
+Lemma tac_twp_alloc Δ s E j K v Φ :
   (∀ l, ∃ Δ',
     envs_app false (Esnoc Enil j (l ↦ v)) Δ = Some Δ' ∧
-    envs_entails Δ' (WP fill K (Lit (LitLoc l)) @ s; E [{ Φ }])) →
-  envs_entails Δ (WP fill K (Alloc e) @ s; E [{ Φ }]).
+    envs_entails Δ' (WP fill K (Val $ LitV l) @ s; E [{ Φ }])) →
+  envs_entails Δ (WP fill K (Alloc v) @ s; E [{ Φ }]).
 Proof.
-  rewrite envs_entails_eq=> ? HΔ.
+  rewrite envs_entails_eq=> HΔ.
   rewrite -twp_bind. eapply wand_apply; first exact: twp_alloc.
   rewrite left_id. apply forall_intro=> l.
   destruct (HΔ l) as (Δ'&?&HΔ'). rewrite envs_app_sound //; simpl.
@@ -176,8 +174,8 @@ Qed.
 Lemma tac_wp_load Δ Δ' s E i K l q v Φ :
   MaybeIntoLaterNEnvs 1 Δ Δ' →
   envs_lookup i Δ' = Some (false, l ↦{q} v)%I →
-  envs_entails Δ' (WP fill K (of_val v) @ s; E {{ Φ }}) →
-  envs_entails Δ (WP fill K (Load (Lit (LitLoc l))) @ s; E {{ Φ }}).
+  envs_entails Δ' (WP fill K (Val v) @ s; E {{ Φ }}) →
+  envs_entails Δ (WP fill K (Load (LitV l)) @ s; E {{ Φ }}).
 Proof.
   rewrite envs_entails_eq=> ???.
   rewrite -wp_bind. eapply wand_apply; first exact: wp_load.
@@ -186,8 +184,8 @@ Proof.
 Qed.
 Lemma tac_twp_load Δ s E i K l q v Φ :
   envs_lookup i Δ = Some (false, l ↦{q} v)%I →
-  envs_entails Δ (WP fill K (of_val v) @ s; E [{ Φ }]) →
-  envs_entails Δ (WP fill K (Load (Lit (LitLoc l))) @ s; E [{ Φ }]).
+  envs_entails Δ (WP fill K (Val v) @ s; E [{ Φ }]) →
+  envs_entails Δ (WP fill K (Load (LitV l)) @ s; E [{ Φ }]).
 Proof.
   rewrite envs_entails_eq=> ??.
   rewrite -twp_bind. eapply wand_apply; first exact: twp_load.
@@ -195,25 +193,23 @@ Proof.
   by apply sep_mono_r, wand_mono.
 Qed.
 
-Lemma tac_wp_store Δ Δ' Δ'' s E i K l v e v' Φ :
-  IntoVal e v' →
+Lemma tac_wp_store Δ Δ' Δ'' s E i K l v v' Φ :
   MaybeIntoLaterNEnvs 1 Δ Δ' →
   envs_lookup i Δ' = Some (false, l ↦ v)%I →
   envs_simple_replace i false (Esnoc Enil i (l ↦ v')) Δ' = Some Δ'' →
-  envs_entails Δ'' (WP fill K (Lit LitUnit) @ s; E {{ Φ }}) →
-  envs_entails Δ (WP fill K (Store (Lit (LitLoc l)) e) @ s; E {{ Φ }}).
+  envs_entails Δ'' (WP fill K (Val $ LitV LitUnit) @ s; E {{ Φ }}) →
+  envs_entails Δ (WP fill K (Store (LitV l) (Val v')) @ s; E {{ Φ }}).
 Proof.
-  rewrite envs_entails_eq=> ?????.
+  rewrite envs_entails_eq=> ????.
   rewrite -wp_bind. eapply wand_apply; first by eapply wp_store.
   rewrite into_laterN_env_sound -later_sep envs_simple_replace_sound //; simpl.
   rewrite right_id. by apply later_mono, sep_mono_r, wand_mono.
 Qed.
-Lemma tac_twp_store Δ Δ' s E i K l v e v' Φ :
-  IntoVal e v' →
+Lemma tac_twp_store Δ Δ' s E i K l v v' Φ :
   envs_lookup i Δ = Some (false, l ↦ v)%I →
   envs_simple_replace i false (Esnoc Enil i (l ↦ v')) Δ = Some Δ' →
-  envs_entails Δ' (WP fill K (Lit LitUnit) @ s; E [{ Φ }]) →
-  envs_entails Δ (WP fill K (Store (Lit (LitLoc l)) e) @ s; E [{ Φ }]).
+  envs_entails Δ' (WP fill K (Val $ LitV LitUnit) @ s; E [{ Φ }]) →
+  envs_entails Δ (WP fill K (Store (LitV l) v') @ s; E [{ Φ }]).
 Proof.
   rewrite envs_entails_eq. intros. rewrite -twp_bind.
   eapply wand_apply; first by eapply twp_store.
@@ -221,121 +217,113 @@ Proof.
   rewrite right_id. by apply sep_mono_r, wand_mono.
 Qed.
 
-Lemma tac_wp_cas Δ Δ' Δ'' s E i K l v e1 v1 e2 v2 Φ :
-  IntoVal e1 v1 → IntoVal e2 v2 →
+Lemma tac_wp_cas Δ Δ' Δ'' s E i K l v v1 v2 Φ :
   MaybeIntoLaterNEnvs 1 Δ Δ' →
   envs_lookup i Δ' = Some (false, l ↦ v)%I →
   envs_simple_replace i false (Esnoc Enil i (l ↦ v2)) Δ' = Some Δ'' →
   vals_cas_compare_safe v v1 →
-  (v = v1 → envs_entails Δ'' (WP fill K (Lit (LitBool true)) @ s; E {{ Φ }})) →
-  (v ≠ v1 → envs_entails Δ' (WP fill K (Lit (LitBool false)) @ s; E {{ Φ }})) →
-  envs_entails Δ (WP fill K (CAS (Lit (LitLoc l)) e1 e2) @ s; E {{ Φ }}).
+  (v = v1 → envs_entails Δ'' (WP fill K (Val $ LitV true) @ s; E {{ Φ }})) →
+  (v ≠ v1 → envs_entails Δ' (WP fill K (Val $ LitV false) @ s; E {{ Φ }})) →
+  envs_entails Δ (WP fill K (CAS (LitV l) (Val v1) (Val v2)) @ s; E {{ Φ }}).
 Proof.
-  rewrite envs_entails_eq=> ?????? Hsuc Hfail. destruct (decide (v = v1)) as [<-|Hne].
+  rewrite envs_entails_eq=> ???? Hsuc Hfail. destruct (decide (v = v1)) as [<-|Hne].
   - rewrite -wp_bind. eapply wand_apply; first exact: wp_cas_suc.
     rewrite into_laterN_env_sound -later_sep /= {1}envs_simple_replace_sound //; simpl.
     apply later_mono, sep_mono_r. rewrite right_id. apply wand_mono; auto.
   - rewrite -wp_bind. eapply wand_apply.
-    { eapply wp_cas_fail; eauto. by eexists. }
+    { eapply wp_cas_fail; eauto. }
     rewrite into_laterN_env_sound -later_sep /= {1}envs_lookup_split //; simpl.
     apply later_mono, sep_mono_r. apply wand_mono; auto.
 Qed.
-Lemma tac_twp_cas Δ Δ' s E i K l v e1 v1 e2 v2 Φ :
-  IntoVal e1 v1 → IntoVal e2 v2 →
+Lemma tac_twp_cas Δ Δ' s E i K l v v1 v2 Φ :
   envs_lookup i Δ = Some (false, l ↦ v)%I →
   envs_simple_replace i false (Esnoc Enil i (l ↦ v2)) Δ = Some Δ' →
   vals_cas_compare_safe v v1 →
-  (v = v1 → envs_entails Δ' (WP fill K (Lit (LitBool true)) @ s; E [{ Φ }])) →
-  (v ≠ v1 → envs_entails Δ (WP fill K (Lit (LitBool false)) @ s; E [{ Φ }])) →
-  envs_entails Δ (WP fill K (CAS (Lit (LitLoc l)) e1 e2) @ s; E [{ Φ }]).
+  (v = v1 → envs_entails Δ' (WP fill K (Val $ LitV true) @ s; E [{ Φ }])) →
+  (v ≠ v1 → envs_entails Δ (WP fill K (Val $ LitV false) @ s; E [{ Φ }])) →
+  envs_entails Δ (WP fill K (CAS (LitV l) v1 v2) @ s; E [{ Φ }]).
 Proof.
-  rewrite envs_entails_eq=> ????? Hsuc Hfail. destruct (decide (v = v1)) as [<-|Hne].
+  rewrite envs_entails_eq=> ??? Hsuc Hfail. destruct (decide (v = v1)) as [<-|Hne].
   - rewrite -twp_bind. eapply wand_apply; first exact: twp_cas_suc.
     rewrite /= {1}envs_simple_replace_sound //; simpl.
     apply sep_mono_r. rewrite right_id. apply wand_mono; auto.
   - rewrite -twp_bind. eapply wand_apply.
-    { eapply twp_cas_fail; eauto. by eexists. }
+    { eapply twp_cas_fail; eauto. }
     rewrite /= {1}envs_lookup_split //; simpl.
     apply sep_mono_r. apply wand_mono; auto.
 Qed.
 
-Lemma tac_wp_cas_fail Δ Δ' s E i K l q v e1 v1 e2 Φ :
-  IntoVal e1 v1 → AsVal e2 →
+Lemma tac_wp_cas_fail Δ Δ' s E i K l q v v1 v2 Φ :
   MaybeIntoLaterNEnvs 1 Δ Δ' →
   envs_lookup i Δ' = Some (false, l ↦{q} v)%I →
   v ≠ v1 → vals_cas_compare_safe v v1 →
-  envs_entails Δ' (WP fill K (Lit (LitBool false)) @ s; E {{ Φ }}) →
-  envs_entails Δ (WP fill K (CAS (Lit (LitLoc l)) e1 e2) @ s; E {{ Φ }}).
+  envs_entails Δ' (WP fill K (Val $ LitV false) @ s; E {{ Φ }}) →
+  envs_entails Δ (WP fill K (CAS (LitV l) v1 v2) @ s; E {{ Φ }}).
 Proof.
-  rewrite envs_entails_eq=> ???????.
+  rewrite envs_entails_eq=> ?????.
   rewrite -wp_bind. eapply wand_apply; first exact: wp_cas_fail.
   rewrite into_laterN_env_sound -later_sep envs_lookup_split //; simpl.
   by apply later_mono, sep_mono_r, wand_mono.
 Qed.
-Lemma tac_twp_cas_fail Δ s E i K l q v e1 v1 e2 Φ :
-  IntoVal e1 v1 → AsVal e2 →
+Lemma tac_twp_cas_fail Δ s E i K l q v v1 v2 Φ :
   envs_lookup i Δ = Some (false, l ↦{q} v)%I →
   v ≠ v1 → vals_cas_compare_safe v v1 →
-  envs_entails Δ (WP fill K (Lit (LitBool false)) @ s; E [{ Φ }]) →
-  envs_entails Δ (WP fill K (CAS (Lit (LitLoc l)) e1 e2) @ s; E [{ Φ }]).
+  envs_entails Δ (WP fill K (Val $ LitV false) @ s; E [{ Φ }]) →
+  envs_entails Δ (WP fill K (CAS (LitV l) v1 v2) @ s; E [{ Φ }]).
 Proof.
   rewrite envs_entails_eq. intros. rewrite -twp_bind.
   eapply wand_apply; first exact: twp_cas_fail.
   rewrite envs_lookup_split //=. by do 2 f_equiv.
 Qed.
 
-Lemma tac_wp_cas_suc Δ Δ' Δ'' s E i K l v e1 v1 e2 v2 Φ :
-  IntoVal e1 v1 → IntoVal e2 v2 →
+Lemma tac_wp_cas_suc Δ Δ' Δ'' s E i K l v v1 v2 Φ :
   MaybeIntoLaterNEnvs 1 Δ Δ' →
   envs_lookup i Δ' = Some (false, l ↦ v)%I →
   envs_simple_replace i false (Esnoc Enil i (l ↦ v2)) Δ' = Some Δ'' →
   v = v1 → val_is_unboxed v →
-  envs_entails Δ'' (WP fill K (Lit (LitBool true)) @ s; E {{ Φ }}) →
-  envs_entails Δ (WP fill K (CAS (Lit (LitLoc l)) e1 e2) @ s; E {{ Φ }}).
+  envs_entails Δ'' (WP fill K (Val $ LitV true) @ s; E {{ Φ }}) →
+  envs_entails Δ (WP fill K (CAS (LitV l) v1 v2) @ s; E {{ Φ }}).
 Proof.
-  rewrite envs_entails_eq=> ????????; subst.
+  rewrite envs_entails_eq=> ??????; subst.
   rewrite -wp_bind. eapply wand_apply.
   { eapply wp_cas_suc; eauto. by left. }
   rewrite into_laterN_env_sound -later_sep envs_simple_replace_sound //; simpl.
   rewrite right_id. by apply later_mono, sep_mono_r, wand_mono.
 Qed.
-Lemma tac_twp_cas_suc Δ Δ' s E i K l v e1 v1 e2 v2 Φ :
-  IntoVal e1 v1 → IntoVal e2 v2 →
+Lemma tac_twp_cas_suc Δ Δ' s E i K l v v1 v2 Φ :
   envs_lookup i Δ = Some (false, l ↦ v)%I →
   envs_simple_replace i false (Esnoc Enil i (l ↦ v2)) Δ = Some Δ' →
   v = v1 → val_is_unboxed v →
-  envs_entails Δ' (WP fill K (Lit (LitBool true)) @ s; E [{ Φ }]) →
-  envs_entails Δ (WP fill K (CAS (Lit (LitLoc l)) e1 e2) @ s; E [{ Φ }]).
+  envs_entails Δ' (WP fill K (Val $ LitV true) @ s; E [{ Φ }]) →
+  envs_entails Δ (WP fill K (CAS (LitV l) v1 v2) @ s; E [{ Φ }]).
 Proof.
-  rewrite envs_entails_eq. intros; subst.
+  rewrite envs_entails_eq=>?????; subst.
   rewrite -twp_bind. eapply wand_apply.
   { eapply twp_cas_suc; eauto. by left. }
   rewrite envs_simple_replace_sound //; simpl.
   rewrite right_id. by apply sep_mono_r, wand_mono.
 Qed.
 
-Lemma tac_wp_faa Δ Δ' Δ'' s E i K l i1 e2 i2 Φ :
-  IntoVal e2 (LitV (LitInt i2)) →
+Lemma tac_wp_faa Δ Δ' Δ'' s E i K l z1 z2 Φ :
   MaybeIntoLaterNEnvs 1 Δ Δ' →
-  envs_lookup i Δ' = Some (false, l ↦ LitV (LitInt i1))%I →
-  envs_simple_replace i false (Esnoc Enil i (l ↦ LitV (LitInt (i1 + i2)))) Δ' = Some Δ'' →
-  envs_entails Δ'' (WP fill K (Lit (LitInt i1)) @ s; E {{ Φ }}) →
-  envs_entails Δ (WP fill K (FAA (Lit (LitLoc l)) e2) @ s; E {{ Φ }}).
+  envs_lookup i Δ' = Some (false, l ↦ LitV z1)%I →
+  envs_simple_replace i false (Esnoc Enil i (l ↦ LitV (z1 + z2))) Δ' = Some Δ'' →
+  envs_entails Δ'' (WP fill K (Val $ LitV z1) @ s; E {{ Φ }}) →
+  envs_entails Δ (WP fill K (FAA (LitV l) (LitV z2)) @ s; E {{ Φ }}).
 Proof.
-  rewrite envs_entails_eq=> ?????; subst.
-  rewrite -wp_bind. eapply wand_apply; first exact: (wp_faa _ _ _ i1 _ i2).
+  rewrite envs_entails_eq=> ????.
+  rewrite -wp_bind. eapply wand_apply; first exact: (wp_faa _ _ _ z1 z2).
   rewrite into_laterN_env_sound -later_sep envs_simple_replace_sound //; simpl.
   rewrite right_id. by apply later_mono, sep_mono_r, wand_mono.
 Qed.
-Lemma tac_twp_faa Δ Δ' s E i K l i1 e2 i2 Φ :
-  IntoVal e2 (LitV (LitInt i2)) →
-  envs_lookup i Δ = Some (false, l ↦ LitV (LitInt i1))%I →
-  envs_simple_replace i false (Esnoc Enil i (l ↦ LitV (LitInt (i1 + i2)))) Δ = Some Δ' →
-  envs_entails Δ' (WP fill K (Lit (LitInt i1)) @ s; E [{ Φ }]) →
-  envs_entails Δ (WP fill K (FAA (Lit (LitLoc l)) e2) @ s; E [{ Φ }]).
+Lemma tac_twp_faa Δ Δ' s E i K l z1 z2 Φ :
+  envs_lookup i Δ = Some (false, l ↦ LitV z1)%I →
+  envs_simple_replace i false (Esnoc Enil i (l ↦ LitV (z1 + z2))) Δ = Some Δ' →
+  envs_entails Δ' (WP fill K (Val $ LitV z1) @ s; E [{ Φ }]) →
+  envs_entails Δ (WP fill K (FAA (LitV l) (LitV z2)) @ s; E [{ Φ }]).
 Proof.
-  rewrite envs_entails_eq=> ????; subst.
-  rewrite -twp_bind. eapply wand_apply; first exact: (twp_faa _ _ _ i1 _ i2).
+  rewrite envs_entails_eq=> ???.
+  rewrite -twp_bind. eapply wand_apply; first exact: (twp_faa _ _ _ z1 z2).
   rewrite envs_simple_replace_sound //; simpl.
   rewrite right_id. by apply sep_mono_r, wand_mono.
 Qed.
@@ -370,15 +358,13 @@ Tactic Notation "wp_alloc" ident(l) "as" constr(H) :=
   lazymatch goal with
   | |- envs_entails _ (wp ?s ?E ?e ?Q) =>
     first
-      [reshape_expr e ltac:(fun K e' =>
-         eapply (tac_wp_alloc _ _ _ _ Htmp K); [iSolveTC|..])
+      [reshape_expr e ltac:(fun K e' => eapply (tac_wp_alloc _ _ _ _ Htmp K))
       |fail 1 "wp_alloc: cannot find 'Alloc' in" e];
     [iSolveTC
     |finish ()]
   | |- envs_entails _ (twp ?s ?E ?e ?Q) =>
     first
-      [reshape_expr e ltac:(fun K e' =>
-         eapply (tac_twp_alloc _ _ _ Htmp K); [iSolveTC|..])
+      [reshape_expr e ltac:(fun K e' => eapply (tac_twp_alloc _ _ _ Htmp K))
       |fail 1 "wp_alloc: cannot find 'Alloc' in" e];
     finish ()
   | _ => fail "wp_alloc: not a 'wp'"
@@ -414,13 +400,12 @@ Tactic Notation "wp_store" :=
     let l := match goal with |- _ = Some (_, (?l ↦{_} _)%I) => l end in
     iAssumptionCore || fail "wp_store: cannot find" l "↦ ?" in
   let finish _ :=
-    wp_expr_simpl; try first [wp_pure (Seq (Lit LitUnit) _)|wp_value_head] in
+    wp_expr_simpl; try first [wp_seq|wp_value_head] in
   iStartProof;
   lazymatch goal with
   | |- envs_entails _ (wp ?s ?E ?e ?Q) =>
     first
-      [reshape_expr e ltac:(fun K e' =>
-         eapply (tac_wp_store _ _ _ _ _ _ K); [iSolveTC|..])
+      [reshape_expr e ltac:(fun K e' => eapply (tac_wp_store _ _ _ _ _ _ K))
       |fail 1 "wp_store: cannot find 'Store' in" e];
     [iSolveTC
     |solve_mapsto ()
@@ -428,8 +413,7 @@ Tactic Notation "wp_store" :=
     |finish ()]
   | |- envs_entails _ (twp ?s ?E ?e ?Q) =>
     first
-      [reshape_expr e ltac:(fun K e' =>
-         eapply (tac_twp_store _ _ _ _ _ K); [iSolveTC|..])
+      [reshape_expr e ltac:(fun K e' => eapply (tac_twp_store _ _ _ _ _ K))
       |fail 1 "wp_store: cannot find 'Store' in" e];
     [solve_mapsto ()
     |pm_reflexivity
@@ -445,8 +429,7 @@ Tactic Notation "wp_cas" "as" simple_intropattern(H1) "|" simple_intropattern(H2
   lazymatch goal with
   | |- envs_entails _ (wp ?s ?E ?e ?Q) =>
     first
-      [reshape_expr e ltac:(fun K e' =>
-         eapply (tac_wp_cas _ _ _ _ _ _ K); [iSolveTC|iSolveTC|..])
+      [reshape_expr e ltac:(fun K e' => eapply (tac_wp_cas _ _ _ _ _ _ K))
       |fail 1 "wp_cas: cannot find 'CAS' in" e];
     [iSolveTC
     |solve_mapsto ()
@@ -456,8 +439,7 @@ Tactic Notation "wp_cas" "as" simple_intropattern(H1) "|" simple_intropattern(H2
     |intros H2; wp_expr_simpl; try wp_value_head]
   | |- envs_entails _ (twp ?E ?e ?Q) =>
     first
-      [reshape_expr e ltac:(fun K e' =>
-         eapply (tac_twp_cas _ _ _ _ _ K); [iSolveTC|iSolveTC|..])
+      [reshape_expr e ltac:(fun K e' => eapply (tac_twp_cas _ _ _ _ _ K))
       |fail 1 "wp_cas: cannot find 'CAS' in" e];
     [solve_mapsto ()
     |pm_reflexivity
@@ -475,8 +457,7 @@ Tactic Notation "wp_cas_fail" :=
   lazymatch goal with
   | |- envs_entails _ (wp ?s ?E ?e ?Q) =>
     first
-      [reshape_expr e ltac:(fun K e' =>
-         eapply (tac_wp_cas_fail _ _ _ _ _ K); [iSolveTC|iSolveTC|..])
+      [reshape_expr e ltac:(fun K e' => eapply (tac_wp_cas_fail _ _ _ _ _ K))
       |fail 1 "wp_cas_fail: cannot find 'CAS' in" e];
     [iSolveTC
     |solve_mapsto ()
@@ -485,8 +466,7 @@ Tactic Notation "wp_cas_fail" :=
     |simpl; try wp_value_head]
   | |- envs_entails _ (twp ?s ?E ?e ?Q) =>
     first
-      [reshape_expr e ltac:(fun K e' =>
-         eapply (tac_twp_cas_fail _ _ _ _ K); [iSolveTC|iSolveTC|..])
+      [reshape_expr e ltac:(fun K e' => eapply (tac_twp_cas_fail _ _ _ _ K))
       |fail 1 "wp_cas_fail: cannot find 'CAS' in" e];
     [solve_mapsto ()
     |try congruence
@@ -503,8 +483,7 @@ Tactic Notation "wp_cas_suc" :=
   lazymatch goal with
   | |- envs_entails _ (wp ?s ?E ?e ?Q) =>
     first
-      [reshape_expr e ltac:(fun K e' =>
-         eapply (tac_wp_cas_suc _ _ _ _ _ _ K); [iSolveTC|iSolveTC|..])
+      [reshape_expr e ltac:(fun K e' => eapply (tac_wp_cas_suc _ _ _ _ _ _ K))
       |fail 1 "wp_cas_suc: cannot find 'CAS' in" e];
     [iSolveTC
     |solve_mapsto ()
@@ -514,8 +493,7 @@ Tactic Notation "wp_cas_suc" :=
     |simpl; try wp_value_head]
   | |- envs_entails _ (twp ?E ?e ?Q) =>
     first
-      [reshape_expr e ltac:(fun K e' =>
-         eapply (tac_twp_cas_suc _ _ _ _ _ K); [iSolveTC|iSolveTC|..])
+      [reshape_expr e ltac:(fun K e' => eapply (tac_twp_cas_suc _ _ _ _ _ K))
       |fail 1 "wp_cas_suc: cannot find 'CAS' in" e];
     [solve_mapsto ()
     |pm_reflexivity
@@ -533,8 +511,7 @@ Tactic Notation "wp_faa" :=
   lazymatch goal with
   | |- envs_entails _ (wp ?s ?E ?e ?Q) =>
     first
-      [reshape_expr e ltac:(fun K e' =>
-         eapply (tac_wp_faa _ _ _ _ _ _ K); [iSolveTC|..])
+      [reshape_expr e ltac:(fun K e' => eapply (tac_wp_faa _ _ _ _ _ _ K))
       |fail 1 "wp_faa: cannot find 'CAS' in" e];
     [iSolveTC
     |solve_mapsto ()
@@ -542,8 +519,7 @@ Tactic Notation "wp_faa" :=
     |wp_expr_simpl; try wp_value_head]
   | |- envs_entails _ (twp ?s ?E ?e ?Q) =>
     first
-      [reshape_expr e ltac:(fun K e' =>
-         eapply (tac_twp_faa _ _ _ _ _ K); [iSolveTC|..])
+      [reshape_expr e ltac:(fun K e' => eapply (tac_twp_faa _ _ _ _ _ K))
       |fail 1 "wp_faa: cannot find 'CAS' in" e];
     [solve_mapsto ()
     |pm_reflexivity
